module and pascal

benchmark/pascal.v
@@ -1,4 +1,4 @@
-Require Import hashtable.
+Require Import hashtable dict module.
 Require Import ZArith Bool.
 Require Import Coq.Numbers.Cyclic.Int63.Uint63.
 
@@ -12,7 +12,8 @@ Fixpoint pascal (n m: nat) : int :=
   | S n', S m' => pascal n' m' + pascal n' m
   end.
 
-Compute pascal 10 5.
+Inductive natnat :=
+  | N : nat -> nat -> natnat.
 
 Fixpoint nat_to_int (n: nat) (acc: int) : int :=
   match n with
@@ -21,19 +22,73 @@ Fixpoint nat_to_int (n: nat) (acc: int) : int :=
   end.
 
 Definition hash (n : nat) (h : int) : int :=
-  nat_to_int n 0 + h.
+  nat_to_int n 0 + h * 345.
 
-Definition hash_couple (n: (nat * nat)) :=
-  let '(n1, n2) := n in
-  hash n1 (hash n2 0).
+Definition eqb_nn (n m: natnat) :=
+  let (n1, n2) := n in
+  let (m1, m2) := m in
+  (n1 =? m1)%nat && (n2 =? m2)%nat.
+
+Theorem eq_spec:
+  forall n m : natnat, reflect (n = m) (eqb_nn n m).
+Proof.
+  intros [n1 n2] [m1 m2]. case (eqb_nn _ _) eqn:H.
+  + apply ReflectT. unfold eqb_nn in H.
+    rewrite andb_true_iff in H. destruct H as [H1 H2].
+    apply Nat.eqb_eq in H1, H2. now rewrite H1, H2.
+  + apply ReflectF. unfold eqb_nn in H.
+    rewrite andb_false_iff in H. destruct H as [H | H];
+    intros H0; rewrite Nat.eqb_neq in H; apply H; 
+    now inversion H0.
+Qed.
 
 
 
-Fixpoint pascal (n m: nat) () : int :=
-  match n, m with
-  | 0, 0 => 1
-  | 0, _ => 0
-  | _, 0 => 1
-  | S n', S m' => pascal n' m' + pascal n' m
-  end.
+Module NATNAT <: Hash_type.
+  Definition A := natnat.
+  Definition eq n m := eqb_nn n m.
+  Definition eq_spec := eq_spec.
+  Definition hashi (i: natnat): int :=
+    let (n1, n2) := i in
+    hash n1 (hash n2 0).
+  Definition hashp (i: natnat): positive :=
+    let hi := hashi i in
+    match to_Z hi with
+    | Z.pos p => p
+    | _ => xH
+    end.
+End NATNAT.
+
+Module Test (H: HashTable NATNAT).
+
+  Fixpoint pascal_memo' (n m: nat) (h: H.t int) : (int * H.t int) :=
+    match H.find h (N n m) with
+    | Some v => (v, h)
+    | None =>
+      match n, m with
+      | 0, 0 => (1, h)
+      | 0, _ => (0, h)
+      | _, 0 => (1, h) 
+      | S n', S m' => 
+        let (v1, h1) := pascal_memo' n' m' h in
+        let (v2, h2) := pascal_memo' n' m h1 in
+        let r := v1 + v2 in
+        (r, H.add h2 (N n m) r) 
+      end
+    end.
+
+  Definition pascal_memo n m :=
+    fst (pascal_memo' n m (H.create 16)).
+
+End Test.
+
+Module HTree := HashTableTree NATNAT.
+Module TestTree := Test HTree.
+
+Module HBucket := HashTableBucket NATNAT.
+Module TestBucket := Test HBucket.
+
+(* Compute pascal 30 15. *)
+Time Compute TestTree.pascal_memo 200 100.
+Time Compute TestBucket.pascal_memo 200 100.
 
